equational_theories/LiftingMagmaFamilies.lean
@@ -1,0 +1,23 @@
+import equational_theories.MagmaLaw
+import equational_theories.Homomorphisms
+
+open Law
+
+class LiftingMagma (G : Type → Type) where
+  instMagma {α} : Magma (G α)
+  ι : ∀ {α}, α → G α
+  lift : ∀ {α}, (α → G α) → (G α →◇ G α)
+  lift_factors : ∀ {α}, ∀ f : α → G α, f = (lift f) ∘ ι
+
+instance {G : Type → Type} [LiftingMagma G] {α : Type} : Magma (G α) := LiftingMagma.instMagma
+
+theorem MagmaLaw.models_iff {α : Type} {G : Type → Type} (law : MagmaLaw α) [LiftingMagma G] :
+    (satisfiesPhi (G := G α) LiftingMagma.ι law) ↔
+    (G α ⊧ law) := by
+  constructor
+  · intro h
+    intro f
+    have := LiftingMagma.lift_factors f
+    rw [this, satisfiesPhi.evalHom, h]
+  · intro h
+    apply h
